\documentclass[10pt]{amsart}
\usepackage{style}

\title[Limits]{Limits Practice\\Math 161}
\date{September 7, 2018}
\author{Blake Farman\\Lafayette College}

\begin{document}
\maketitle

\makenameslot

In each of the problems, evaluate the limit if it exists.  
Indicate any limit laws that you use.
If the limit does not exist, explain why.
\begin{thm}
  Use the limits
  \[\lim_{x \to 2} f(x) = 4 \qquad \lim_{x\to 2} g(x) = -2\qquad \lim_{x\to2} h(x) = 0\]
  to complete each of the following.

  \begin{enumerate}[(a)]
  \item
    \(\displaystyle{\lim_{x \to 2} [f(x) + 5g(x)]}\)
    \vspace{1in}
  \item
    \(\displaystyle{\lim_{x \to 2} \left[g(x)\right]^3}\)
    \vspace{1in}
  \item
    \(\displaystyle{\lim_{x \to 2} \sqrt{f(x)}}\)
    \vspace{1in}
  \item
    \(\displaystyle{\lim_{x \to 2} \frac{3f(x)}{g(x)}}\)
    \vspace{1in}
  \item
    \(\displaystyle{\lim_{x \to 2} \frac{g(x)}{h(x)}}\)
    \vspace{1in}
  \item
    \(\displaystyle{\lim_{x \to 2} \frac{g(x)h(x)}{f(x)}}\)
    \vspace{1in}

  \end{enumerate}
\end{thm}

\begin{thm}
  \(\displaystyle{\lim_{x \to -1}(x^4 - 3x)(x^2 + 5x + 3)}\)
\end{thm}

\vspace{1in}

\begin{thm}
  \(\displaystyle{\lim_{u \to -2} \sqrt{u^4 + 3u + 6}}\)
\end{thm}

\vspace{1in}

\begin{thm}
  \(\displaystyle{\lim_{t \to 2} \left(\frac{t^2 - 2}{t^3 - 3t + 5}\right)^2}\)
\end{thm}

\vspace{1in}

\begin{thm}
  \(\displaystyle{\lim_{t \to -3} \frac{t^2 - 9}{2t^2 + 7t + 3}}\)\\
\end{thm}

\vspace{1in}
\begin{thm}
  \(\displaystyle{\lim_{x \to -3} \frac{x^2 + 3x}{x^2 - x - 12}}\)
\end{thm}

\vspace{1in}

\begin{thm}
  \(\displaystyle{\lim_{x \to -2} \frac{x + 2}{x^3 + 8}}\)

  \noindent [Hint: \(x^3 + a^3 = (x + a)(x - ax + a^2)\)]
\end{thm}

\vspace{1in}

\begin{thm}
  \(\displaystyle{\lim_{h \to 0} \frac{(2 + h)^3 - 8}{h}}\)
\end{thm}

\vspace{1in}

\begin{thm}
  \(\displaystyle{\lim_{t \to 0} \left(\frac{1}{t} - \frac{1}{t^2 + t}\right)}\)
\end{thm}

\vspace{1in}

\begin{thm}
  \(\displaystyle{\lim_{t \to 0} \left(\frac{\sqrt{1 + t} - \sqrt{1 - t}}{t}\right)}\)
\end{thm}

\vspace{1in}
\begin{thm}
  \(\displaystyle{\lim_{h \to 0} \frac{\frac{1}{(x + h)^2} - \frac{1}{x^2}}{h}}\)
\end{thm}
\end{document}

