\documentclass[10pt]{amsart}
\usepackage{style}

\title[Product and Quotient]{Product and Quotient Rules}
\date{September 17, 2018}
\author{Blake Farman}
\address{Lafayette College}

\begin{document}
\maketitle

\makenameslot

In each of the problems, use the derivative rules to differentiate the given function.
Use proper notation and simplify your final answers.
In some cases it might be advantageous to simplify/rewrite first.
Do not use rules found in later sections.

\begin{multicols}{2}
  \begin{thm}
    \(\displaystyle{f(x) = \left(1 + \sqrt{x}\right) x^3}\)
  \end{thm}

  \vspace{1.25in}

  \begin{thm}
    \(\displaystyle{g(t) = \left(\frac{2}{t} + t^5\right)(t^3 + 1)}\)
  \end{thm}

  \vspace{1.25in}

  \begin{thm}
    \(\displaystyle{h(y) = \frac{1}{y^3 + 2y + 1}}\)
  \end{thm}

  \vspace{1.25in}
  
  \begin{thm}
    \(\displaystyle{y = \frac{1}{x + \sqrt{x}}}\)
  \end{thm}

  \vspace{1.25in}
  
  \begin{thm}
    \(\displaystyle{g(z) = \frac{z^2 + 1}{z^3 - 5}}\)
  \end{thm}

  \vspace{1.25in}
  
  \begin{thm}
    \(\displaystyle{y = \frac{\sqrt{x}}{x^3 + 1}}\)
  \end{thm}

  \vspace{1.25in}
\end{multicols}

\newpage
\begin{multicols}{2}
  \begin{thm}
    \(\displaystyle{z = \frac{t^2}{(t - 4)(2 - t^3)}}\)
  \end{thm}

  \begin{thm}
    \(\displaystyle{h(x) = \frac{\left(x^3 + 1\right)\sqrt{x}}{x^2}}\)
  \end{thm}
\end{multicols}

\vspace{1.25in}

\begin{thm}
  Let \(f(x) = g(x)h(x)\), \(g(10) = -4\), \(h(10) = 560\), \(g^\prime(10) = 0\), \(h^\prime(10) = 4\).
  Find \(f^\prime(10)\).
\end{thm}

\vspace{2in}

\begin{thm}
  Let \(z(-3) = 6\), \(z^\prime(-3) = 15\), and
  \[y(x) = \frac{z(x)}{1 + x^2}.\]
  Find \(y^\prime(-3)\).
\end{thm}
\end{document}

